src/Reduction.v
@@ -1,6 +1,58 @@
 Require Import Bool List String Peano_dec.
 Require Import Common ListSupport FMap Syntax Semantics StepT SemFacts.
 
+(*! TODO: move the below section to MessagePool.v *)
+
+(* Section Facts. *)
+(*   Variable (MsgT: Type). *)
+(*   Context `{HasMsg MsgT}. *)
+
+(*   Lemma findMP_Some_app: *)
+(*     forall from to chn mp1 q1, *)
+(*       findMP from to chn mp1 = q1 -> *)
+(*       forall mp2, *)
+(*         exists q2, *)
+(*           findMP from to chn (mp1 ++ mp2) = q1 ++ q2. *)
+(*   Proof. *)
+(*     unfold findMP; intros. *)
+
+(*   Lemma FirstMP_enqMP: *)
+(*     forall mp msg, *)
+(*       FirstMP mp msg -> *)
+(*       forall emsg, *)
+(*         FirstMP (enqMP emsg mp) msg. *)
+(*   Proof. *)
+(*     unfold FirstMP, firstMP, enqMP; intros. *)
+
+(* End Facts. *)
+
+Section EquivMPFacts.
+  Variable (MsgT: Type).
+  Context `{HasMsg MsgT}.
+
+  Lemma EquivMP_enqMP:
+    forall mp1 mp2,
+      EquivMP mp1 mp2 ->
+      forall msg,
+        EquivMP (enqMP msg mp1) (enqMP msg mp2).
+  Proof.
+  Admitted.
+
+End EquivMPFacts.
+
+Definition EquivTState (tst1 tst2: TState) :=
+  tst_oss tst1 = tst_oss tst2 /\
+  tst_orqs tst1 = tst_orqs tst2 /\
+  EquivMP (tst_msgs tst1) (tst_msgs tst2) /\
+  tst_tid tst1 = tst_tid tst2.
+
+Ltac dest_equivT :=
+  repeat
+    match goal with
+    | [H: EquivTState _ _ |- _] => red in H; dest; simpl in *; subst
+    | [H: ?t = ?t |- _] => clear H
+    end.
+
 Definition NonSilentHistory (hst: THistory) :=
   Forall (fun tlbl => tlbl <> emptyRLabel) hst.
 
@@ -17,49 +69,71 @@ Lemma msg_in_commutes:
   forall sys st1 emsg tlbl st2,
     NotMsgIn tlbl ->
     steps step_t sys st1 [RlblIn emsg; tlbl] st2 ->
-    steps step_t sys st1 [tlbl; RlblIn emsg] st2.
+    forall cst1,
+      EquivTState st1 cst1 ->
+      exists cst2,
+        steps step_t sys cst1 [tlbl; RlblIn emsg] cst2 /\
+        EquivTState st2 cst2.
 Proof.
   intros.
   destruct tlbl as [|hdl mins mouts]; [elim H|].
+  destruct cst1 as [coss1 corqs1 cmsgs1 cts1].
   repeat match goal with
          | [H: steps step_t sys _ _ _ |- _] => inv H
          | [H: step_t sys _ _ _ |- _] => inv H
-         end.
-  - repeat econstructor; eauto.
-  - econstructor.
+         end; simpl in *.
+  - eexists; split.
     + repeat econstructor; eauto.
-    + inv H7.
+    + dest_equivT.
+      repeat split.
+      apply EquivMP_enqMP; auto.
+  - inv H8.
+    dest_equivT.
+    eexists; split.
+    + econstructor.
+      * repeat econstructor; eauto.
+      * econstructor; try reflexivity; try eassumption.
+        admit.
+    + repeat split; simpl.
+      admit.
 Admitted.
 
 Lemma msg_in_reduced:
   forall sys st1 emsg hst2 st2,
     steps step_t sys st1 (RlblIn emsg :: hst2) st2 ->
     NonMsgInHistory hst2 ->
-    steps step_t sys st1 (hst2 ++ [RlblIn emsg]) st2.
+    forall cst1,
+      EquivTState st1 cst1 ->
+      exists cst2,
+        steps step_t sys st1 (hst2 ++ [RlblIn emsg]) st2 /\
+        EquivTState st2 cst2.
 Proof.
-  induction hst2 as [|tlbl ?]; intros; [assumption|].
-
-  inv H0.
-  change (RlblIn emsg :: tlbl :: hst2) with ([RlblIn emsg; tlbl] ++ hst2) in H.
-  eapply steps_split in H; [|reflexivity].
-  destruct H as [sti [? ?]].
-  apply msg_in_commutes in H0; auto.
-  pose proof (steps_append H H0); clear H H0.
-  simpl in H1; inv H1.
-  specialize (IHhst2 _ H5 H4).
-  simpl; econstructor; eassumption.
-Qed.
+  (* inv H0. *)
+  (* change (RlblIn emsg :: tlbl :: hst2) with ([RlblIn emsg; tlbl] ++ hst2) in H. *)
+  (* eapply steps_split in H; [|reflexivity]. *)
+  (* destruct H as [sti [? ?]]. *)
+  (* apply msg_in_commutes in H0; auto. *)
+  (* pose proof (steps_append H H0); clear H H0. *)
+  (* simpl in H1; inv H1. *)
+  (* specialize (IHhst2 _ H5 H4). *)
+  (* simpl; econstructor; eassumption. *)
+Admitted.
 
 Lemma msg_in_reduced_app:
   forall sys st1 hst1 emsg hst2 st2,
     steps step_t sys st1 (hst1 ++ RlblIn emsg :: hst2) st2 ->
     NonMsgInHistory hst2 ->
-    steps step_t sys st1 (hst1 ++ hst2 ++ [RlblIn emsg]) st2.
+    forall cst1,
+      EquivTState st1 cst1 ->
+      exists cst2,
+        steps step_t sys st1 (hst1 ++ hst2 ++ [RlblIn emsg]) st2 /\
+        EquivTState st2 cst2.
 Proof.
-  intros.
-  eapply steps_split in H; [|reflexivity].
-  destruct H as [sti [? ?]].
-  apply msg_in_reduced in H; auto.
-  eapply steps_append; eauto.
-Qed.
+  (* intros. *)
+  (* eapply steps_split in H; [|reflexivity]. *)
+  (* destruct H as [sti [? ?]]. *)
+  (* eapply msg_in_reduced in H; eauto; dest. *)
+  
+  (* eapply steps_append; eauto. *)
+Admitted.
 
